MEM is relocated to the WB instr

model/agp32EnvironmentScript.sml
@@ -84,6 +84,7 @@ val is_mem_def = Define `
   (accessors.get_command (step n) = 0w /\ (fext (n-1)).ready ==>
    (fext n).mem = (fext (n-1)).mem /\
    (fext n).inst_rdata = (fext (n-1)).inst_rdata /\
+   (fext n).data_rdata = (fext (n-1)).data_rdata /\
    (fext n).ready) /\
 
   (* Read instruction *)
@@ -91,6 +92,7 @@ val is_mem_def = Define `
    ?m. (!p. p < m ==> (fext (n + p)).mem = (fext (n-1)).mem /\ ~(fext (n + p)).ready) /\
        (fext (n + m)).mem = (fext (n-1)).mem /\
        (fext (n + m)).inst_rdata = word_at_addr (fext n).mem (align_addr (accessors.get_PC (step n))) /\
+       (fext (n + m)).data_rdata = (fext (n + m - 1)).data_rdata /\
        (fext (n + m)).ready) /\
 
   (* Read instruction + read data *)
@@ -108,6 +110,7 @@ val is_mem_def = Define `
         (let newmem = mem_update (fext (n-1)).mem (align_addr (accessors.get_data_addr (step n))) (accessors.get_data_wdata (step n)) (accessors.get_data_wstrb (step n)) in
          (fext (n + m)).mem = newmem /\
          (fext (n + m)).inst_rdata = word_at_addr newmem (align_addr (accessors.get_PC (step n))) /\
+         (fext (n + m)).data_rdata = (fext (n + m - 1)).data_rdata /\
          (fext (n + m)).ready)) /\
 
  (* Clear cache block used for printing ... exactly the same semantics as "read instruction" *)
@@ -115,6 +118,7 @@ val is_mem_def = Define `
    ?m. (!p. p < m ==> (fext (n + p)).mem = (fext (n-1)).mem /\ ~(fext (n + p)).ready) /\
        (fext (n + m)).mem = (fext (n-1)).mem /\
        (fext (n + m)).inst_rdata = word_at_addr (fext n).mem (align_addr (accessors.get_PC (step n))) /\
+       (fext (n + m)).data_rdata = (fext (n + m - 1)).data_rdata /\
        (fext (n + m)).ready) /\
  
  (* Nothing in the beginning, exists a request internally *)
