proof/agp32CorrectScript.sml
@@ -74,6 +74,7 @@ Proof
    cheat >-
    cheat >-
    cheat >-
+   cheat >-
    (** fext not ready, fetch disabled **)
    fs [enable_stg_def,not_fext_ready_and_agp32_IF_PC_write_disable] >-
    (** fext not ready, decode disabled **)
